Revise the simulation relation for reordering stores/updates

src/opt/FulfillStep.v
@@ -29,7 +29,8 @@ Set Implicit Arguments.
 Inductive fulfill_step (lc1:Local.t) (sc1:TimeMap.t) (loc:Loc.t) (from to:Time.t) (val:Const.t) (releasedm released:Capability.t) (ord:Ordering.t): forall (lc2:Local.t) (sc2:TimeMap.t), Prop :=
 | step_fulfill
     promises2
-    (RELEASED: released = Capability.join releasedm ((Commit.write_commit lc1.(Local.commit) sc1 loc to ord).(Commit.rel) loc))
+    (REL_LE: Capability.le (Capability.join releasedm ((Commit.write_commit lc1.(Local.commit) sc1 loc to ord).(Commit.rel) loc)) released)
+    (REL_WF: Capability.wf released)
     (WRITABLE: Commit.writable lc1.(Local.commit) sc1 loc to ord)
     (REMOVE: Memory.remove lc1.(Local.promises) loc from to val released promises2)
     (TIME: Time.lt from to):
@@ -58,24 +59,6 @@ Proof.
   - apply CommitFacts.write_sc_incr.
 Qed.
 
-Lemma fulfill_write
-      lc1 sc1 mem1 loc from to val releasedm released ord lc2 sc2
-      (FULFILL: fulfill_step lc1 sc1 loc from to val releasedm released ord lc2 sc2)
-      (REL_WF: Capability.wf releasedm)
-      (REL_CLOSED: Memory.closed_capability releasedm mem1)
-      (ORD: Ordering.le ord Ordering.relaxed)
-      (WF1: Local.wf lc1 mem1)
-      (SC1: Memory.closed_timemap sc1 mem1)
-      (MEM1: Memory.closed mem1):
-  Local.write_step lc1 sc1 mem1 loc from to val releasedm released ord lc2 sc2 mem1 Memory.promise_kind_lower.
-Proof.
-  inv FULFILL. econs; eauto.
-  - econs; eauto. apply Memory.promise_exists_same; try apply WF1; auto.
-    + repeat (try condtac; committac; try apply WF1).
-    + eapply Memory.remove_get0. eauto.
-  - i. destruct ord; inv ORD; inv H.
-Qed.
-
 Lemma write_promise_fulfill
       lc0 sc0 mem0 loc from to val releasedm released ord lc2 sc2 mem2 kind
       (WRITE: Local.write_step lc0 sc0 mem0 loc from to val releasedm released ord lc2 sc2 mem2 kind)
@@ -87,6 +70,10 @@ Lemma write_promise_fulfill
   exists lc1,
     <<STEP1: Local.promise_step lc0 mem0 loc from to val released lc1 mem2 kind>> /\
     <<STEP2: fulfill_step lc1 sc0 loc from to val releasedm released ord lc2 sc2>> /\
+    <<REL: released = Capability.join releasedm
+             (Commit.rel
+               (Commit.write_commit (Local.commit lc0) sc0 loc to ord)
+               loc)>> /\
     <<ORD: Ordering.le Ordering.acqrel ord ->
            Local.promises lc0 loc = Cell.bot /\
            kind = Memory.promise_kind_add>>.
@@ -94,8 +81,32 @@ Proof.
   exploit Local.write_step_future; eauto. i. des.
   inv WRITE. inv WRITE0. esplits; eauto.
   - econs; eauto.
-  - refine (step_fulfill _ _ _ _ _); auto.
-    eapply promise_time_lt. eauto.
+  - refine (step_fulfill _ _ _ _ _ _); auto.
+    + refl.
+    + eapply promise_time_lt. eauto.
+Qed.
+
+Lemma fulfill_write
+      lc1 sc1 mem1 loc from to val releasedm released ord lc2 sc2
+      (FULFILL: fulfill_step lc1 sc1 loc from to val releasedm released ord lc2 sc2)
+      (REL_WF: Capability.wf releasedm)
+      (REL_CLOSED: Memory.closed_capability releasedm mem1)
+      (ORD: Ordering.le ord Ordering.relaxed)
+      (WF1: Local.wf lc1 mem1)
+      (SC1: Memory.closed_timemap sc1 mem1)
+      (MEM1: Memory.closed mem1):
+  exists released' mem2',
+    <<STEP: Local.write_step lc1 sc1 mem1 loc from to val releasedm released' ord lc2 sc2 mem2' Memory.promise_kind_lower>> /\
+    <<REL_LE: Capability.le released' released>> /\
+    <<MEM: Memory.sim mem1 mem2'>>.
+Proof.
+  inv FULFILL.
+  exploit remove_promise_remove; try exact REMOVE; eauto; try apply WF1.
+  { repeat (try condtac; committac; try apply WF1). }
+  i. des.
+  esplits; eauto. econs; eauto.
+  - econs; eauto.
+  - i. destruct ord; inv ORD; inv H.
 Qed.
 
 Lemma promise_fulfill_write
@@ -109,8 +120,41 @@ Lemma promise_fulfill_write
       (WF0: Local.wf lc0 mem0)
       (SC0: Memory.closed_timemap sc0 mem0)
       (MEM0: Memory.closed mem0):
-  Local.write_step lc0 sc0 mem0 loc from to val releasedm released ord lc2 sc2 mem2 kind.
+  exists released' mem2',
+    <<STEP: Local.write_step lc0 sc0 mem0 loc from to val releasedm released' ord lc2 sc2 mem2' kind>> /\
+    <<REL_LE: Capability.le released' released>> /\
+    <<MEM: Memory.sim mem2 mem2'>>.
 Proof.
+  exploit Local.promise_step_future; eauto. i. des.
   inv PROMISE. inv FULFILL.
-  refine (Local.step_write _ _ _ _ _); auto. econs; eauto.
+  exploit remove_promise_remove; try exact REMOVE; eauto; try apply WF2.
+  { repeat (try condtac; committac; try apply WF2). }
+  i. des.
+  esplits; eauto.
+  refine (Local.step_write _ _ _ _ _); eauto.
+  econs; eauto.
+  admit. (* promise_kind + promise_lower <= promise_kind *)
+Admitted.
+
+Lemma promise_fulfill_write_exact
+      lc0 sc0 mem0 loc from to val releasedm released ord lc1 lc2 sc2 mem2 kind
+      (PROMISE: Local.promise_step lc0 mem0 loc from to val released lc1 mem2 kind)
+      (FULFILL: fulfill_step lc1 sc0 loc from to val releasedm released ord lc2 sc2)
+      (REL_WF: Capability.wf releasedm)
+      (REL_CLOSED: Memory.closed_capability releasedm mem0)
+      (REL: released = Capability.join releasedm
+              (Commit.rel
+                (Commit.write_commit (Local.commit lc0) sc0 loc to ord)
+                loc))
+      (ORD: Ordering.le Ordering.acqrel ord -> lc0.(Local.promises) loc = Cell.bot /\
+                                              kind = Memory.promise_kind_add)
+      (WF0: Local.wf lc0 mem0)
+      (SC0: Memory.closed_timemap sc0 mem0)
+      (MEM0: Memory.closed mem0):
+         Local.write_step lc0 sc0 mem0 loc from to val releasedm released ord lc2 sc2 mem2 kind.
+Proof.
+  exploit Local.promise_step_future; eauto. i. des.
+  inv PROMISE. inv FULFILL.
+  refine (Local.step_write _ _ _ _ _); eauto.
+  econs; eauto.
 Qed.
